term/term-project.v
@@ -1,0 +1,1224 @@
+(* term-project.v *)
+(* FPP 2020 - YSC3236 2020-2021, Sem1 *)
+(* Olivier Danvy <danvy@yale-nus.edu.sg> *)
+(* Version of 15 Nov 2020 *)
+
+(* ********** *)
+
+(* Three language processors for arithmetic expressions. *)
+
+(*
+   name: Bobbie Soedirgo
+   student ID number: A0181001A
+   e-mail address: sram-b@comp.nus.edu.sg
+*)
+
+(* ********** *)
+
+(*
+
+The primary goal of this term project is to prove the following theorem:
+
+  Theorem the_commutative_diagram :
+    forall sp : source_program,
+      interpret sp = run (compile sp).
+
+for
+
+* a source language of arithmetic expressions:
+
+    Inductive arithmetic_expression : Type :=
+    | Literal : nat -> arithmetic_expression
+    | Plus : arithmetic_expression -> arithmetic_expression -> arithmetic_expression
+    | Minus : arithmetic_expression -> arithmetic_expression -> arithmetic_expression.
+    
+    Inductive source_program : Type :=
+    | Source_program : arithmetic_expression -> source_program.
+
+* a target language of byte-code instructions:
+
+    Inductive byte_code_instruction : Type :=
+    | PUSH : nat -> byte_code_instruction
+    | ADD : byte_code_instruction
+    | SUB : byte_code_instruction.
+    
+    Inductive target_program : Type :=
+    | Target_program : list byte_code_instruction -> target_program.
+
+* a semantics of expressible values:
+
+    Inductive expressible_value : Type :=
+    | Expressible_nat : nat -> expressible_value
+    | Expressible_msg : string -> expressible_value.
+
+* a source interpreter
+
+    interpret : source_program -> expressible_value
+
+* a compiler
+
+    compile : source_program -> target_program
+
+* a target interpreter
+
+    run : target_program -> expressible_value
+
+The source for errors is subtraction,
+since subtracting two natural numbers does not always yield a natural number:
+for example, 3 - 2 is defined but not 2 - 3.
+
+You are expected, at the very least:
+
+* to implement a source interpreter
+  and to verify that it satisfies its specification
+
+* to implement a target interpreter (i.e., a virtual machine)
+  and to verify that it satisfies its specification
+
+* to implement a compiler
+  and to verify that it satisfies its specification
+
+* to prove that the diagram commutes, i.e., to show that
+  interpreting any given expression
+  gives the same result as
+  compiling this expression and then running the resulting compiled program
+
+Beyond this absolute minimum, in decreasing importance, it would be good:
+
+* to make a copy of the above in a separate file
+  and modify it mutatis mutandis
+  so that the three language processors operate from right to left instead of from left to right,
+
+* to write an accumulator-based compiler and to prove that it satisfies the specification,
+
+* to investigate byte-code verification,
+
+* to investigate decompilation, and
+
+* if there is any time left, to prove that each of the specifications specifies a unique function.
+
+Also, feel free to expand the source language and the target language,
+e.g., with multiplication, quotient, and modulo.
+
+*)
+
+(* ********** *)
+
+Ltac fold_unfold_tactic name := intros; unfold name; fold name; reflexivity.
+  
+Require Import Arith Bool List String Ascii.
+
+(* caution: only use natural numbers up to 5000 *)
+Definition string_of_nat (q0 : nat) : string :=
+  let s0 := String (ascii_of_nat (48 + (q0 mod 10))) EmptyString
+  in if q0 <? 10
+     then s0
+     else let q1 := q0 / 10
+          in let s1 := String (ascii_of_nat (48 + (q1 mod 10))) s0
+             in if q1 <? 10
+                then s1
+                else let q2 := q1 / 10
+                     in let s2 := String (ascii_of_nat (48 + (q2 mod 10))) s1
+                        in if q2 <? 10
+                           then s2
+                           else let q3 := q2 / 10
+                                in let s2 := String (ascii_of_nat (48 + (q3 mod 10))) s2
+                        in if q3 <? 10
+                           then s2
+                           else "00000".
+
+Notation "A =n= B" := (beq_nat A B) (at level 70, right associativity).
+
+(* ********** *)
+
+(* Arithmetic expressions: *)
+
+Inductive arithmetic_expression : Type :=
+| Literal : nat -> arithmetic_expression
+| Plus : arithmetic_expression -> arithmetic_expression -> arithmetic_expression
+| Minus : arithmetic_expression -> arithmetic_expression -> arithmetic_expression.
+
+(* Source programs: *)
+
+Inductive source_program : Type :=
+| Source_program : arithmetic_expression -> source_program.
+
+(* ********** *)
+
+(* Semantics: *)
+
+Inductive expressible_value : Type :=
+| Expressible_nat : nat -> expressible_value
+| Expressible_msg : string -> expressible_value.
+
+(* ********** *)
+
+Definition specification_of_evaluate (evaluate : arithmetic_expression -> expressible_value) :=
+  (forall n : nat,
+     evaluate (Literal n) = Expressible_nat n)
+  /\
+  ((forall (ae1 ae2 : arithmetic_expression)
+           (s1 : string),
+       evaluate ae1 = Expressible_msg s1 ->
+       evaluate (Plus ae1 ae2) = Expressible_msg s1)
+   /\
+   (forall (ae1 ae2 : arithmetic_expression)
+           (n1 : nat)
+           (s2 : string),
+       evaluate ae1 = Expressible_nat n1 ->
+       evaluate ae2 = Expressible_msg s2 ->
+       evaluate (Plus ae1 ae2) = Expressible_msg s2)
+   /\
+   (forall (ae1 ae2 : arithmetic_expression)
+           (n1 n2 : nat),
+       evaluate ae1 = Expressible_nat n1 ->
+       evaluate ae2 = Expressible_nat n2 ->
+       evaluate (Plus ae1 ae2) = Expressible_nat (n1 + n2)))
+  /\
+  ((forall (ae1 ae2 : arithmetic_expression)
+           (s1 : string),
+       evaluate ae1 = Expressible_msg s1 ->
+       evaluate (Minus ae1 ae2) = Expressible_msg s1)
+   /\
+   (forall (ae1 ae2 : arithmetic_expression)
+           (n1 : nat)
+           (s2 : string),
+       evaluate ae1 = Expressible_nat n1 ->
+       evaluate ae2 = Expressible_msg s2 ->
+       evaluate (Minus ae1 ae2) = Expressible_msg s2)
+   /\
+   (forall (ae1 ae2 : arithmetic_expression)
+           (n1 n2 : nat),
+       evaluate ae1 = Expressible_nat n1 ->
+       evaluate ae2 = Expressible_nat n2 ->
+       n1 <? n2 = true ->
+       evaluate (Minus ae1 ae2) = Expressible_msg (String.append "numerical underflow: -" (string_of_nat (n2 - n1))))
+   /\
+   (forall (ae1 ae2 : arithmetic_expression)
+           (n1 n2 : nat),
+       evaluate ae1 = Expressible_nat n1 ->
+       evaluate ae2 = Expressible_nat n2 ->
+       n1 <? n2 = false ->
+       evaluate (Minus ae1 ae2) = Expressible_nat (n1 - n2))).
+
+Theorem there_is_at_most_one_evaluate_function :
+  forall (evaluate1 evaluate2 : arithmetic_expression -> expressible_value),
+    specification_of_evaluate evaluate1 ->
+    specification_of_evaluate evaluate2 ->
+    forall ae : arithmetic_expression,
+      evaluate1 ae = evaluate2 ae.
+Proof.
+Admitted.
+
+Definition specification_of_interpret (interpret : source_program -> expressible_value) :=
+  forall evaluate : arithmetic_expression -> expressible_value,
+    specification_of_evaluate evaluate ->
+    forall ae : arithmetic_expression,
+      interpret (Source_program ae) = evaluate ae.
+
+Theorem there_is_at_most_one_interpret_function :
+  forall (interpret1 interpret2 : source_program -> expressible_value),
+    specification_of_interpret interpret1 ->
+    specification_of_interpret interpret2 ->
+    forall sp : source_program,
+      interpret1 sp = interpret2 sp.
+Proof.
+Admitted.
+
+(* Task 1: 
+   a. time permitting, prove that each of the definitions above specifies at most one function;
+   b. implement these two functions; and
+   c. verify that each of your functions satisfies its specification.
+*)
+
+Fixpoint evaluate_v0 (ae : arithmetic_expression) : expressible_value :=
+  match ae with
+  | Literal n =>
+    Expressible_nat n
+  | Plus ae1 ae2 =>
+    match evaluate_v0 ae1 with
+    | Expressible_nat n1 =>
+      match evaluate_v0 ae2 with
+      | Expressible_nat n2 =>
+        Expressible_nat (n1 + n2)
+      | Expressible_msg s2 =>
+        Expressible_msg s2
+      end
+    | Expressible_msg s1 =>
+      Expressible_msg s1
+    end
+  | Minus ae1 ae2 =>
+    match evaluate_v0 ae1 with
+    | Expressible_nat n1 =>
+      match evaluate_v0 ae2 with
+      | Expressible_nat n2 =>
+        if n1 <? n2
+        then Expressible_msg (String.append "numerical underflow: -" (string_of_nat (n2 - n1)))
+        else Expressible_nat (n1 - n2)
+      | Expressible_msg s2 =>
+        Expressible_msg s2
+      end
+    | Expressible_msg s1 =>
+      Expressible_msg s1
+    end
+  end.
+
+Lemma fold_unfold_evaluate_v0_Literal :
+  forall (n : nat),
+    evaluate_v0 (Literal n) = Expressible_nat n.
+Proof.
+  fold_unfold_tactic evaluate_v0.
+Qed.
+
+Lemma fold_unfold_evaluate_v0_Plus :
+  forall (ae1 ae2 : arithmetic_expression),
+    evaluate_v0 (Plus ae1 ae2) =
+    match evaluate_v0 ae1 with
+    | Expressible_nat n1 =>
+      match evaluate_v0 ae2 with
+      | Expressible_nat n2 =>
+        Expressible_nat (n1 + n2)
+      | Expressible_msg s2 =>
+        Expressible_msg s2
+      end
+    | Expressible_msg s1 =>
+      Expressible_msg s1
+    end.
+Proof.
+  fold_unfold_tactic evaluate_v0.
+Qed.
+
+Lemma fold_unfold_evaluate_v0_Minus :
+  forall (ae1 ae2 : arithmetic_expression),
+    evaluate_v0 (Minus ae1 ae2) =
+    match evaluate_v0 ae1 with
+    | Expressible_nat n1 =>
+      match evaluate_v0 ae2 with
+      | Expressible_nat n2 =>
+        if n1 <? n2
+        then Expressible_msg (String.append "numerical underflow: -" (string_of_nat (n2 - n1)))
+        else Expressible_nat (n1 - n2)
+      | Expressible_msg s2 =>
+        Expressible_msg s2
+      end
+    | Expressible_msg s1 =>
+      Expressible_msg s1
+    end.
+Proof.
+  fold_unfold_tactic evaluate_v0.
+Qed.
+
+Theorem evaluate_v0_satisfies_the_specification_of_evaluate :
+  specification_of_evaluate evaluate_v0.
+Proof.
+  unfold specification_of_evaluate.
+  split.
+  - exact fold_unfold_evaluate_v0_Literal.
+  - split.
+    + split.
+      * intros ae1 ae2 s1 H1_msg.
+        rewrite fold_unfold_evaluate_v0_Plus.
+        rewrite H1_msg.
+        reflexivity.
+      * split.
+        -- intros ae1 ae2 n1 s2 H1_nat H2_msg.
+           rewrite fold_unfold_evaluate_v0_Plus.
+           rewrite H1_nat.
+           rewrite H2_msg.
+           reflexivity.
+        -- intros ae1 ae2 n1 n2 H1_nat H2_nat.
+           rewrite fold_unfold_evaluate_v0_Plus.
+           rewrite H1_nat.
+           rewrite H2_nat.
+           reflexivity.
+    + split.
+      * intros ae1 ae2 s1 H1_msg.
+        rewrite fold_unfold_evaluate_v0_Minus.
+        rewrite H1_msg.
+        reflexivity.
+      * split.
+        -- intros ae1 ae2 n1 s2 H1_nat H2_msg.
+           rewrite fold_unfold_evaluate_v0_Minus.
+           rewrite H1_nat.
+           rewrite H2_msg.
+           reflexivity.
+        -- split.
+           ++ intros ae1 ae2 n1 n2 H1_nat H2_nat H_lt.
+              rewrite fold_unfold_evaluate_v0_Minus.
+              rewrite H1_nat.
+              rewrite H2_nat.
+              rewrite H_lt.
+              reflexivity.
+           ++ intros ae1 ae2 n1 n2 H1_nat H2_nat H_gt.
+              rewrite fold_unfold_evaluate_v0_Minus.
+              rewrite H1_nat.
+              rewrite H2_nat.
+              rewrite H_gt.
+              reflexivity.
+Qed.
+
+Definition interpret_v0 (sp : source_program) : expressible_value :=
+  match sp with
+  | Source_program ae =>
+    evaluate_v0 ae
+  end.
+
+Theorem interpret_v0_satisfies_the_specification_of_interpret :
+  specification_of_interpret interpret_v0.
+Proof.
+  unfold specification_of_interpret, interpret_v0.
+  intros evaluate' S_evaluate' ae.
+  Check (there_is_at_most_one_evaluate_function evaluate_v0 evaluate' evaluate_v0_satisfies_the_specification_of_evaluate S_evaluate' ae).
+  exact (there_is_at_most_one_evaluate_function evaluate_v0 evaluate' evaluate_v0_satisfies_the_specification_of_evaluate S_evaluate' ae).
+Qed.
+
+(* ********** *)
+
+(* Byte-code instructions: *)
+
+Inductive byte_code_instruction : Type :=
+| PUSH : nat -> byte_code_instruction
+| ADD : byte_code_instruction
+| SUB : byte_code_instruction.
+
+(* Target programs: *)
+
+Inductive target_program : Type :=
+| Target_program : list byte_code_instruction -> target_program.
+
+(* Data stack: *)
+
+Definition data_stack := list nat.
+
+(* ********** *)
+
+Inductive result_of_decoding_and_execution : Type :=
+| OK : data_stack -> result_of_decoding_and_execution
+| KO : string -> result_of_decoding_and_execution.
+
+Definition specification_of_decode_execute (decode_execute : byte_code_instruction -> data_stack -> result_of_decoding_and_execution) :=
+  (forall (n : nat)
+          (ds : data_stack),
+     decode_execute (PUSH n) ds = OK (n :: ds))
+  /\
+  ((decode_execute ADD nil = KO "ADD: stack underflow")
+   /\
+   (forall (n2 : nat),
+       decode_execute ADD (n2 :: nil) = KO "ADD: stack underflow")
+   /\
+   (forall (n1 n2 : nat)
+           (ds : data_stack),
+       decode_execute ADD (n2 :: n1 :: ds) = OK ((n1 + n2) :: ds)))
+  /\
+  ((decode_execute SUB nil = KO "SUB: stack underflow")
+   /\
+   (forall (n2 : nat),
+       decode_execute SUB (n2 :: nil) = KO "SUB: stack underflow")
+   /\
+   (forall (n1 n2 : nat)
+           (ds : data_stack),
+       n1 <? n2 = true ->
+       decode_execute SUB (n2 :: n1 :: ds) = KO (String.append "numerical underflow: -" (string_of_nat (n2 - n1))))
+   /\
+   (forall (n1 n2 : nat)
+           (ds : data_stack),
+       n1 <? n2 = false ->
+       decode_execute SUB (n2 :: n1 :: ds) = OK ((n1 - n2) :: ds))).
+
+Theorem there_is_at_most_one_decode_execute_function :
+  forall (decode_execute1 decode_execute2 : byte_code_instruction -> data_stack -> result_of_decoding_and_execution),
+    specification_of_decode_execute decode_execute1 ->
+    specification_of_decode_execute decode_execute2 ->
+    forall (bci : byte_code_instruction)
+      (ds : data_stack),
+      decode_execute1 bci ds = decode_execute2 bci ds.
+Proof.
+Admitted.
+
+(* Task 2:
+   a. time permitting, prove that the definition above specifies at most one function;
+   b. implement this function; and
+   c. verify that your function satisfies the specification.
+*)
+
+Definition decode_execute_v0 (bcis : byte_code_instruction) (ds : data_stack) : result_of_decoding_and_execution :=
+  match bcis with
+  | PUSH n =>
+    OK (n :: ds)
+  | ADD =>
+    match ds with
+    | nil =>
+      KO "ADD: stack underflow"
+    | n2 :: ds' =>
+      match ds' with
+      | nil =>
+      KO "ADD: stack underflow"
+      | n1 :: ds'' =>
+        OK ((n1 + n2) :: ds'')
+      end
+    end
+  | SUB =>
+    match ds with
+    | nil =>
+      KO "SUB: stack underflow"
+    | n2 :: ds' =>
+      match ds' with
+      | nil =>
+      KO "SUB: stack underflow"
+      | n1 :: ds'' =>
+        if n1 <? n2
+        then KO (String.append "numerical underflow: -" (string_of_nat (n2 - n1)))
+        else OK ((n1 - n2) :: ds'')
+      end
+    end
+  end.
+    
+Theorem decode_execute_v0_satisfies_the_specification_of_decode_execute :
+  specification_of_decode_execute decode_execute_v0.
+Proof.
+  unfold specification_of_decode_execute, decode_execute_v0.
+  split.
+  - reflexivity.
+  - split.
+    + split.
+      * reflexivity.
+      * split.
+        -- reflexivity.
+        -- reflexivity.
+    + split.
+      * reflexivity.
+      * split.
+        -- reflexivity.
+        -- split.
+           ++ intros.
+              rewrite H.
+              reflexivity.
+           ++ intros.
+              rewrite H.
+              reflexivity.
+Qed.
+
+(* ********** *)
+
+(* Specification of the virtual machine: *)
+
+Definition specification_of_fetch_decode_execute_loop (fetch_decode_execute_loop : list byte_code_instruction -> data_stack -> result_of_decoding_and_execution) :=
+  forall decode_execute : byte_code_instruction -> data_stack -> result_of_decoding_and_execution,
+    specification_of_decode_execute decode_execute ->
+    (forall ds : data_stack,
+        fetch_decode_execute_loop nil ds = OK ds)
+    /\
+    (forall (bci : byte_code_instruction)
+            (bcis' : list byte_code_instruction)
+            (ds ds' : data_stack),
+        decode_execute bci ds = OK ds' ->
+        fetch_decode_execute_loop (bci :: bcis') ds =
+        fetch_decode_execute_loop bcis' ds')
+    /\
+    (forall (bci : byte_code_instruction)
+            (bcis' : list byte_code_instruction)
+            (ds : data_stack)
+            (s : string),
+        decode_execute bci ds = KO s ->
+        fetch_decode_execute_loop (bci :: bcis') ds =
+        KO s).
+
+Theorem there_is_at_most_one_fetch_decode_execute_loop_function :
+  forall (fetch_decode_execute_loop1 fetch_decode_execute_loop2 : list byte_code_instruction -> data_stack -> result_of_decoding_and_execution),
+    specification_of_fetch_decode_execute_loop fetch_decode_execute_loop1 ->
+    specification_of_fetch_decode_execute_loop fetch_decode_execute_loop2 ->
+    forall (bcis : list byte_code_instruction)
+      (ds : data_stack),
+      fetch_decode_execute_loop1 bcis ds = fetch_decode_execute_loop2 bcis ds.
+Proof.
+Admitted.
+
+(* Task 3:
+   a. time permitting, prove that the definition above specifies at most one function;
+   b. implement this function; and
+   c. verify that your function satisfies the specification.
+*)
+
+Fixpoint fetch_decode_execute_loop_v0 (bcis : list byte_code_instruction) (ds : data_stack) : result_of_decoding_and_execution :=
+  match bcis with
+  | nil =>
+    OK ds
+  | bci :: bcis' =>
+    match decode_execute_v0 bci ds with
+    | OK ds' =>
+      fetch_decode_execute_loop_v0 bcis' ds'
+    | KO s =>
+      KO s
+    end
+  end.
+
+Lemma fold_unfold_fetch_decode_execute_loop_v0_nil :
+  forall ds : data_stack,
+    fetch_decode_execute_loop_v0 nil ds =
+    OK ds.
+Proof.
+  fold_unfold_tactic fetch_decode_execute_loop_v0.
+Qed.
+
+Lemma fold_unfold_fetch_decode_execute_loop_v0_cons :
+  forall (bci : byte_code_instruction)
+    (bcis' : list byte_code_instruction)
+    (ds : data_stack),
+    fetch_decode_execute_loop_v0 (bci :: bcis') ds =
+    match decode_execute_v0 bci ds with
+    | OK ds' =>
+      fetch_decode_execute_loop_v0 bcis' ds'
+    | KO s =>
+      KO s
+    end.
+Proof.
+  fold_unfold_tactic fetch_decode_execute_loop_v0.
+Qed.
+
+Theorem fetch_decode_execute_loop_v0_satisfies_the_specification_of_fetch_decode_execute_loop :
+  specification_of_fetch_decode_execute_loop fetch_decode_execute_loop_v0.
+Proof.
+  unfold specification_of_fetch_decode_execute_loop.
+  intros decode_execute S_decode_execute.
+  split.
+  (* bcis: nil case *)
+  - exact fold_unfold_fetch_decode_execute_loop_v0_nil.
+  (* bcis: cons case *)
+  - split. 
+    (* decode_execute: OK case *)
+    (* + intros [n | |] bcis'. *)
+    + intros bci bcis' ds ds' H_decode_execute.
+      rewrite fold_unfold_fetch_decode_execute_loop_v0_cons.
+      rewrite (there_is_at_most_one_decode_execute_function
+                 decode_execute
+                 decode_execute_v0
+                 S_decode_execute
+                 decode_execute_v0_satisfies_the_specification_of_decode_execute
+                 bci
+                 ds) in H_decode_execute.
+      rewrite H_decode_execute.
+      reflexivity.
+    + 
+
+      
+      (* bci: PUSH case *)
+      * intros ds ds' H_decode_execute.
+        rewrite fold_unfold_fetch_decode_execute_loop_v0_cons.
+        unfold decode_execute_v0.
+        destruct S_decode_execute as [S_decode_execute _].
+        rewrite S_decode_execute in H_decode_execute.
+        injection H_decode_execute as H_ds.
+        rewrite H_ds.
+        reflexivity.
+      (* bci: ADD case *)
+      * intros [| n2 [| n1 ds']] ds'' H_decode_execute.
+        (* ds: nil case *)
+        -- destruct S_decode_execute as [_ [[S_decode_execute _] _]].
+           rewrite S_decode_execute in H_decode_execute.
+           discriminate H_decode_execute.
+        (* ds: n2 :: nil case *)
+        -- destruct S_decode_execute as [_ [[_ [S_decode_execute _]] _]].
+           rewrite S_decode_execute in H_decode_execute.
+           discriminate H_decode_execute.
+        (* ds: n2 :: n1 :: nil case *)
+        -- destruct S_decode_execute as [_ [[_ [_ S_decode_execute]] _]].
+           rewrite S_decode_execute in H_decode_execute.
+           rewrite fold_unfold_fetch_decode_execute_loop_v0_cons.
+           unfold decode_execute_v0.
+           injection H_decode_execute as H.
+           rewrite H.
+           reflexivity.
+      (* bci: SUB case *)
+      * intros [| n2 [| n1 ds']] ds'' H_decode_execute.
+        (* ds: nil case *)
+        -- destruct S_decode_execute as [_ [_ [H _]]].
+           rewrite H in H_decode_execute.
+           discriminate H_decode_execute.
+        (* ds: n2 :: nil case *)
+        -- destruct S_decode_execute as [_ [_ [_ [H _]]]].
+           rewrite H in H_decode_execute.
+           discriminate H_decode_execute.
+        (* ds: n2 :: n1 :: nil case *)
+        -- case (n1 <? n2) eqn:H_n.
+           ++ destruct S_decode_execute as [_ [_ [_ [_ [H _]]]]].
+              rewrite (H n1 n2 ds' H_n) in H_decode_execute.
+              discriminate H_decode_execute.
+           ++ destruct S_decode_execute as [_ [_ [_ [_ [_ H]]]]].
+              rewrite (H n1 n2 ds' H_n) in H_decode_execute.
+              injection H_decode_execute as H_n_sub.
+              rewrite fold_unfold_fetch_decode_execute_loop_v0_cons.
+              unfold decode_execute_v0.
+              rewrite H_n.
+              rewrite H_n_sub.
+              reflexivity.
+    (* decode_execute: KO case *)
+    + intros [n | |] bcis'.
+      (* bci: PUSH case *)
+      * intros ds s H_decode_execute.
+        destruct S_decode_execute as [S_decode_execute _].
+        rewrite S_decode_execute in H_decode_execute.
+        discriminate H_decode_execute.
+      (* bci: ADD case *)
+      * intros [| n2 [| n1 ds']] ds'' H_decode_execute.
+        (* ds: nil case *)
+        -- destruct S_decode_execute as [_ [[S_decode_execute _] _]].
+           rewrite S_decode_execute in H_decode_execute.
+           rewrite fold_unfold_fetch_decode_execute_loop_v0_cons.
+           unfold decode_execute_v0.
+           exact H_decode_execute.
+        (* ds: n2 :: nil case *)
+        -- destruct S_decode_execute as [_ [[_ [S_decode_execute _]] _]].
+           rewrite S_decode_execute in H_decode_execute.
+           rewrite fold_unfold_fetch_decode_execute_loop_v0_cons.
+           unfold decode_execute_v0.
+           exact H_decode_execute.
+        (* ds: n2 :: n1 :: nil case *)
+        -- destruct S_decode_execute as [_ [[_ [_ S_decode_execute]] _]].
+           rewrite S_decode_execute in H_decode_execute.
+           discriminate H_decode_execute.
+      (* bci: SUB case *)
+      * intros [| n2 [| n1 ds']] ds'' H_decode_execute.
+        (* ds: nil case *)
+        -- destruct S_decode_execute as [_ [_ [S_decode_execute _]]].
+           rewrite S_decode_execute in H_decode_execute.
+           rewrite fold_unfold_fetch_decode_execute_loop_v0_cons.
+           unfold decode_execute_v0.
+           exact H_decode_execute.
+        (* ds: n2 :: nil case *)
+        -- destruct S_decode_execute as [_ [_ [_ [S_decode_execute _]]]].
+           rewrite S_decode_execute in H_decode_execute.
+           rewrite fold_unfold_fetch_decode_execute_loop_v0_cons.
+           unfold decode_execute_v0.
+           exact H_decode_execute.
+        (* ds: n2 :: n1 :: nil case *)
+        -- case (n1 <? n2) eqn:H_n.
+           ++ destruct S_decode_execute as [_ [_ [_ [_ [H _]]]]].
+              rewrite (H n1 n2 ds' H_n) in H_decode_execute.
+              rewrite fold_unfold_fetch_decode_execute_loop_v0_cons.
+              unfold decode_execute_v0.
+              rewrite H_n.
+              exact H_decode_execute.
+           ++ destruct S_decode_execute as [_ [_ [_ [_ [_ H]]]]].
+              rewrite (H n1 n2 ds' H_n) in H_decode_execute.
+              discriminate H_decode_execute.
+Qed.
+
+(* ********** *)
+
+(* Task 4:
+   Prove that for any lists of byte-code instructions bcis1 and bcis2,
+   and for any data stack ds,
+   executing the concatenation of bcis1 and bcis2 (i.e., bcis1 ++ bcis2) with ds
+   gives the same result as
+   (1) executing bcis1 with ds, and then
+   (2) executing bcis2 with the resulting data stack, if there exists one.
+*)
+
+Lemma fold_unfold_append_nil :
+  forall bcis2 : list byte_code_instruction,
+    nil ++ bcis2 = bcis2.
+Proof.
+  fold_unfold_tactic List.app.
+Qed.
+
+Lemma fold_unfold_append_cons :
+  forall (bci1 : byte_code_instruction)
+         (bci1s bci2s : list byte_code_instruction),
+    (bci1 :: bci1s) ++ bci2s =
+    bci1 :: (bci1s ++ bci2s).
+Proof.
+  fold_unfold_tactic List.app.
+Qed.
+
+Proposition fetch_decode_execute_loop_v0_and_append_commute :
+  forall (bcis1 bcis2 : list byte_code_instruction)
+         (ds1 : data_stack),
+    (forall (ds2 : data_stack),
+       fetch_decode_execute_loop_v0 bcis1 ds1 = OK ds2 ->
+       fetch_decode_execute_loop_v0 (bcis1 ++ bcis2) ds1 = fetch_decode_execute_loop_v0 bcis2 ds2)
+    /\
+    (forall (s : string),
+       fetch_decode_execute_loop_v0 bcis1 ds1 = KO s ->
+       fetch_decode_execute_loop_v0 (bcis1 ++ bcis2) ds1 = KO s).
+Proof.
+  intro bcis1.
+  induction bcis1 as [| bci1 bcis1' IH1].
+  (* bcis1: nil *)
+  - intros bcis2 ds1.
+    split.
+    (* OK *)
+    + intros ds2 H_fdel.
+      rewrite fold_unfold_append_nil.
+      rewrite fold_unfold_fetch_decode_execute_loop_v0_nil in H_fdel.
+      injection H_fdel as H_ds.
+      rewrite H_ds.
+      reflexivity.
+    (* KO *)
+    + intros s H_fdel.
+      rewrite fold_unfold_fetch_decode_execute_loop_v0_nil in H_fdel.
+      discriminate H_fdel.
+  (* bcis1: cons *)
+  - split.
+    (* OK *)
+    + intros ds2 H_fdel.
+      rewrite fold_unfold_fetch_decode_execute_loop_v0_cons in H_fdel.
+      rewrite fold_unfold_append_cons.
+      rewrite fold_unfold_fetch_decode_execute_loop_v0_cons.
+      case bci1 as [n | |].
+      (* bci: PUSH *)
+      * unfold decode_execute_v0 in H_fdel.
+        unfold decode_execute_v0.
+        destruct (IH1 bcis2 (n :: ds1)) as [H _].
+        exact (H ds2 H_fdel).
+      (* bci: ADD *)
+      * unfold decode_execute_v0 in H_fdel.
+        unfold decode_execute_v0.
+        case ds1 as [| n2 [| n1 ds']].
+        -- discriminate H_fdel.
+        -- discriminate H_fdel.
+        -- destruct (IH1 bcis2 (n1 + n2 :: ds')) as [H _].
+           exact (H ds2 H_fdel).
+      (* bci: SUB *)
+      * unfold decode_execute_v0 in H_fdel.
+        unfold decode_execute_v0.
+        case ds1 as [| n2 [| n1 ds1']].
+        -- discriminate H_fdel.
+        -- discriminate H_fdel.
+        -- case (n1 <? n2) eqn:H_n.
+           ++ discriminate H_fdel.
+           ++ destruct (IH1 bcis2 (n1 - n2 :: ds1')) as [H _].
+              exact (H ds2 H_fdel).
+    (* KO *)
+    + intros s H_fdel.
+      rewrite fold_unfold_fetch_decode_execute_loop_v0_cons in H_fdel.
+      rewrite fold_unfold_append_cons.
+      rewrite fold_unfold_fetch_decode_execute_loop_v0_cons.
+      case bci1 as [n | |].
+      (* bci1: PUSH *)
+      * unfold decode_execute_v0 in H_fdel.
+        unfold decode_execute_v0.
+        destruct (IH1 bcis2 (n :: ds1)) as [_ H].
+        exact (H s H_fdel).
+      (* bci: ADD *)
+      * unfold decode_execute_v0 in H_fdel.
+        unfold decode_execute_v0.
+        case ds1 as [| n2 [| n1 ds1']].
+        -- exact H_fdel.
+        -- exact H_fdel.
+        -- destruct (IH1 bcis2 (n1 + n2 :: ds1')) as [_ H].
+           exact (H s H_fdel).
+      (* bci: SUB *)
+      * unfold decode_execute_v0 in H_fdel.
+        unfold decode_execute_v0.
+        case ds1 as [| n2 [| n1 ds1']].
+        -- exact H_fdel.
+        -- exact H_fdel.
+        -- case (n1 <? n2) eqn:H_n.
+           ++ exact H_fdel.
+           ++ destruct (IH1 bcis2 (n1 - n2 :: ds1')) as [_ H].
+              exact (H s H_fdel).
+Qed.
+
+(* ********** *)
+
+Definition specification_of_run (run : target_program -> expressible_value) :=
+  forall fetch_decode_execute_loop : list byte_code_instruction -> data_stack -> result_of_decoding_and_execution,
+    specification_of_fetch_decode_execute_loop fetch_decode_execute_loop ->
+    (forall (bcis : list byte_code_instruction),
+       fetch_decode_execute_loop bcis nil = OK nil ->
+       run (Target_program bcis) = Expressible_msg "no result on the data stack")
+    /\
+    (forall (bcis : list byte_code_instruction)
+            (n : nat),
+       fetch_decode_execute_loop bcis nil = OK (n :: nil) ->
+       run (Target_program bcis) = Expressible_nat n)
+    /\
+    (forall (bcis : list byte_code_instruction)
+            (n n' : nat)
+            (ds'' : data_stack),
+       fetch_decode_execute_loop bcis nil = OK (n :: n' :: ds'') ->
+       run (Target_program bcis) = Expressible_msg "too many results on the data stack")
+    /\
+    (forall (bcis : list byte_code_instruction)
+            (s : string),
+       fetch_decode_execute_loop bcis nil = KO s ->
+       run (Target_program bcis) = Expressible_msg s).
+
+Theorem there_is_at_most_one_run_function :
+  forall (run1 run2 : target_program -> expressible_value),
+    specification_of_run run1 ->
+    specification_of_run run2 ->
+    forall tp : target_program,
+      run1 tp = run2 tp.
+Proof.
+Admitted.
+
+(* Task 5:
+   a. time permitting, prove that the definition above specifies at most one function;
+   b. implement this function; and
+   c. verify that your function satisfies the specification.
+*)
+
+Definition run_v0 (tp : target_program) : expressible_value :=
+  match tp with
+  | Target_program bcis =>
+    match fetch_decode_execute_loop_v0 bcis nil with
+    | OK ds =>
+      match ds with
+      | nil =>
+        Expressible_msg "no result on the data stack"
+      | n :: ds' =>
+        match ds' with
+        | nil =>
+          Expressible_nat n
+        | n' :: ds'' =>
+          Expressible_msg "too many results on the data stack"
+        end
+      end
+    | KO s =>
+      Expressible_msg s
+    end
+  end.
+
+
+Theorem run_v0_satisfies_the_specification_of_run :
+  specification_of_run run_v0.
+Proof.
+  unfold specification_of_run, run_v0.
+  intros fdel S_fdel.
+  split.
+  (* fdel: OK nil *)
+  - intro bcis.
+    induction bcis as [| bci bcis' IH].
+    + intro H_fdel.
+      rewrite fold_unfold_fetch_decode_execute_loop_v0_nil.
+      reflexivity.
+    + intro H_fdel.
+      rewrite fold_unfold_fetch_decode_execute_loop_v0_cons.
+      unfold decode_execute_v0.
+      case bci as [n | |].
+      (* bci: PUSH *)
+      * destruct (S_fdel
+                    decode_execute_v0
+                    decode_execute_v0_satisfies_the_specification_of_decode_execute) as [_ [H _]].
+        unfold decode_execute_v0 in H.
+        rewrite (H (PUSH n) bcis' nil nil) in H_fdel.
+        admit.
+        admit.
+      (* bci: ADD *)
+      * admit.
+      (* bci: SUB *)
+      * admit.
+  - split.
+    (* fdel: OK (n2 :: nil) *)
+     + admit.
+     + split.
+       (* fdel: OK (n2 :: n1 :: nil) *)
+       * admit.
+       (* fdel: KO *)
+       * admit.
+Admitted.
+
+(* ********** *)
+
+Definition specification_of_compile_aux (compile_aux : arithmetic_expression -> list byte_code_instruction) :=
+  (forall n : nat,
+     compile_aux (Literal n) = PUSH n :: nil)
+  /\
+  (forall ae1 ae2 : arithmetic_expression,
+     compile_aux (Plus ae1 ae2) = (compile_aux ae1) ++ (compile_aux ae2) ++ (ADD :: nil))
+  /\
+  (forall ae1 ae2 : arithmetic_expression,
+     compile_aux (Minus ae1 ae2) = (compile_aux ae1) ++ (compile_aux ae2) ++ (SUB :: nil)).
+
+Theorem there_is_at_most_one_compile_aux_function :
+  forall (compile_aux1 compile_aux2 : arithmetic_expression -> list byte_code_instruction),
+    specification_of_compile_aux compile_aux1 ->
+    specification_of_compile_aux compile_aux2 ->
+    forall ae : arithmetic_expression,
+      compile_aux1 ae = compile_aux2 ae.
+Proof.
+Admitted.
+
+(* Task 6:
+   a. time permitting, prove that the definition above specifies at most one function;
+   b. implement this function using list concatenation, i.e., ++; and
+   c. verify that your function satisfies the specification.
+*)
+
+Fixpoint compile_v0_aux (ae : arithmetic_expression) : list byte_code_instruction :=
+  match ae with
+  | Literal n =>
+    PUSH n :: nil
+  | Plus ae1  ae2 =>
+    (compile_v0_aux ae1) ++ (compile_v0_aux ae2) ++ (ADD :: nil)
+  | Minus ae1 ae2 =>
+    (compile_v0_aux ae1) ++ (compile_v0_aux ae2) ++ (SUB :: nil)
+  end.
+
+Compute compile_v0_aux (Plus (Literal 1) (Minus (Literal 2) (Literal 3))).
+
+Lemma fold_unfold_compile_v0_aux_Literal :
+  forall (n : nat),
+    compile_v0_aux (Literal n) =
+    PUSH n :: nil.
+Proof.
+  fold_unfold_tactic compile_v0_aux.
+Qed.
+
+Lemma fold_unfold_compile_v0_aux_Plus :
+  forall (ae1 ae2 : arithmetic_expression),
+    compile_v0_aux (Plus ae1 ae2) =
+    (compile_v0_aux ae1) ++ (compile_v0_aux ae2) ++ (ADD :: nil).
+Proof.
+  fold_unfold_tactic compile_v0_aux.
+Qed.
+
+Lemma fold_unfold_compile_v0_aux_Minus :
+  forall (ae1 ae2 : arithmetic_expression),
+    compile_v0_aux (Minus ae1 ae2) =
+    (compile_v0_aux ae1) ++ (compile_v0_aux ae2) ++ (SUB :: nil).
+Proof.
+  fold_unfold_tactic compile_v0_aux.
+Qed.
+
+Theorem compile_v0_aux_satisfies_the_specification_of_compile_aux :
+  specification_of_compile_aux compile_v0_aux.
+Proof.
+Admitted.
+
+Definition specification_of_compile (compile : source_program -> target_program) :=
+  forall compile_aux : arithmetic_expression -> list byte_code_instruction,
+    specification_of_compile_aux compile_aux ->
+    forall ae : arithmetic_expression,
+      compile (Source_program ae) = Target_program (compile_aux ae).
+
+Theorem there_is_at_most_one_compile_function :
+  forall (compile1 compile2 : source_program -> target_program),
+    specification_of_compile compile1 ->
+    specification_of_compile compile2 ->
+    forall sp : source_program,
+      compile1 sp = compile2 sp.
+Proof.
+Admitted.
+
+(* Task 7:
+   a. time permitting, prove that the definition above specifies at most one function;
+   b. implement this function; and
+   c. verify that your function satisfies the specification.
+*)
+
+Definition compile_v0 (sp : source_program) : target_program :=
+  match sp with
+  | Source_program ae =>
+    Target_program (compile_v0_aux ae)
+  end.
+
+Theorem compile_v0_satisfies_the_specification_of_compile :
+  specification_of_compile compile_v0.
+Proof.
+Admitted.
+
+(* Task 8:
+   implement an alternative compiler
+   using an auxiliary function with an accumulator
+   and that does not use ++ but :: instead,
+   and prove that it satisfies the specification.
+
+   Subsidiary question:
+   Are your compiler and your alternative compiler equivalent?
+   How can you tell?
+*)
+
+Fixpoint compile_v1_aux_aux (ae : arithmetic_expression) (bcis : list byte_code_instruction) : list byte_code_instruction :=
+  match ae with
+  | Literal n =>
+    PUSH n :: bcis
+  | Plus ae1 ae2 =>
+    compile_v1_aux_aux ae1 (compile_v1_aux_aux ae2 (ADD :: bcis))
+  | Minus ae1 ae2 =>
+    compile_v1_aux_aux ae1 (compile_v1_aux_aux ae2 (SUB :: bcis))
+  end.
+
+Compute compile_v1_aux_aux (Plus (Literal 1) (Minus (Literal 2) (Literal 3))) nil.
+
+Lemma fold_unfold_compile_v1_aux_aux_Literal :
+  forall (n : nat)
+    (bcis : list byte_code_instruction),
+    compile_v1_aux_aux (Literal n) bcis =
+    PUSH n :: bcis.
+Proof.
+  fold_unfold_tactic compile_v1_aux_aux.
+Qed.
+
+Lemma fold_unfold_compile_v1_aux_aux_Plus :
+  forall (ae1 ae2 : arithmetic_expression)
+    (bcis : list byte_code_instruction),
+    compile_v1_aux_aux (Plus ae1 ae2) bcis =
+    compile_v1_aux_aux ae1 (compile_v1_aux_aux ae2 (ADD :: bcis)).
+Proof.
+  fold_unfold_tactic compile_v1_aux_aux.
+Qed.
+
+Lemma fold_unfold_compile_v1_aux_aux_Minus :
+  forall (ae1 ae2 : arithmetic_expression)
+    (bcis : list byte_code_instruction),
+    compile_v1_aux_aux (Minus ae1 ae2) bcis =
+    compile_v1_aux_aux ae1 (compile_v1_aux_aux ae2 (SUB :: bcis)).
+Proof.
+  fold_unfold_tactic compile_v1_aux_aux.
+Qed.
+
+Definition compile_v1_aux (ae : arithmetic_expression) : list byte_code_instruction :=
+  compile_v1_aux_aux ae nil.
+
+Theorem compile_v1_aux_satisfies_the_specification_of_compile_aux :
+  specification_of_compile_aux compile_v1_aux.
+Proof.
+  unfold specification_of_compile_aux, compile_v1_aux.
+  split.
+  - intro n.
+    rewrite fold_unfold_compile_v1_aux_aux_Literal.
+    reflexivity.
+  - split.
+    (* Plus case *)
+    + admit.
+    (* Minus case *)
+    + admit.
+Admitted.
+
+Definition compile_v1 (sp : source_program) : target_program :=
+  match sp with
+  | Source_program ae =>
+    Target_program (compile_v1_aux ae)
+  end.
+
+(* ********** *)
+
+(* Task 9 (the capstone):
+   Prove that interpreting an arithmetic expression gives the same result
+   as first compiling it and then executing the compiled program.
+*)
+
+Lemma about_the_commutative_diagram :
+  forall ae : arithmetic_expression,
+    (exists n : nat,
+        evaluate_v0 ae = Expressible_nat n
+        /\
+        fetch_decode_execute_loop_v0 (compile_v0_aux ae) nil = OK (n :: nil))
+    \/
+    (exists s : string,
+        evaluate_v0 ae = Expressible_msg s
+        /\
+        fetch_decode_execute_loop_v0 (compile_v0_aux ae) nil = KO s).
+Proof.
+  intro ae.
+  induction ae as [n |
+                   ae1 [[n1 [IH1_i IH1_c]] | [s1 [IH1_i IH1_c]]] ae2 [[n2 [IH2_i IH2_c]] | [s2 [IH2_i IH2_c]]] |
+                   ae1 [[n1 [IH1_i IH1_c]] | [s1 [IH1_i IH1_c]]] ae2 [[n2 [IH2_i IH2_c]] | [s2 [IH2_i IH2_c]]]].
+  (* Literal *)
+  - left.
+    exists n.
+    split.
+    + rewrite fold_unfold_evaluate_v0_Literal.
+      reflexivity.
+    + rewrite fold_unfold_compile_v0_aux_Literal.
+      rewrite fold_unfold_fetch_decode_execute_loop_v0_cons.
+      unfold decode_execute_v0.
+      exact (fold_unfold_fetch_decode_execute_loop_v0_nil (n :: nil)).
+  (* Plus nat nat *)
+  - admit.
+  (* Plus nat msg *)
+  - right.
+    exists s2.
+    rewrite fold_unfold_evaluate_v0_Plus.
+    split.
+    + rewrite IH1_i.
+      rewrite IH2_i.
+      reflexivity.
+    + rewrite fold_unfold_compile_v0_aux_Plus.
+      destruct (fetch_decode_execute_loop_v0_and_append_commute
+                  (compile_v0_aux ae1)
+                  (compile_v0_aux ae2 ++ ADD :: nil)
+                  nil) as [H _].
+      rewrite (H (n1 :: nil) IH1_c).
+      destruct (fetch_decode_execute_loop_v0_and_append_commute
+                  (compile_v0_aux ae2)
+                  (ADD :: nil)
+                  (n1 :: nil)) as [_ H1].
+      apply (H1 s2).
+  (* Plus msg nat *)
+  - right.
+    exists s1.
+    rewrite fold_unfold_evaluate_v0_Plus.
+    split.
+    + rewrite IH1_i.
+      reflexivity.
+    + rewrite fold_unfold_compile_v0_aux_Plus.
+      destruct (fetch_decode_execute_loop_v0_and_append_commute
+                  (compile_v0_aux ae1)
+                  (compile_v0_aux ae2 ++ ADD :: nil)
+                  nil) as [_ H].
+      apply (H s1).
+      exact IH1_c.
+  (* Plus msg msg *)
+  - right.
+    exists s1.
+    rewrite fold_unfold_evaluate_v0_Plus.
+    split.
+    + rewrite IH1_i.
+      reflexivity.
+    + rewrite fold_unfold_compile_v0_aux_Plus.
+      destruct (fetch_decode_execute_loop_v0_and_append_commute
+                  (compile_v0_aux ae1)
+                  (compile_v0_aux ae2 ++ ADD :: nil)
+                  nil) as [_ H].
+      apply (H s1).
+      exact IH1_c.
+  (* Minus nat nat *)
+  - admit.
+  (* Minus nat msg *)
+  - admit.
+  (* Minus msg nat *)
+  - admit.
+  (* Minus msg msg *)
+  - admit.
+Admitted.
+
+Theorem the_commutative_diagram :
+  forall (sp : source_program),
+    interpret_v0 sp = run_v0 (compile_v0 sp).
+Proof.
+  intros [ae].
+  unfold interpret_v0, run_v0, compile_v0.
+  destruct (about_the_commutative_diagram ae) as [[n [H_nat_i H_nat_c]] | [s [H_msg_i H_msg_c]]].
+  - rewrite H_nat_i.
+    rewrite H_nat_c.
+    reflexivity.
+  - rewrite H_msg_i.
+    rewrite H_msg_c.
+    reflexivity.
+Qed.
+
+(* Theorem the_commutative_diagram : *)
+(*   forall (sp : source_program), *)
+(*     interpret_v0 sp = run_v0 (compile_v0 sp). *)
+(* Proof. *)
+(*   unfold interpret_v0, run_v0, compile_v0. *)
+(*   intros [ae]. *)
+(*   induction ae as [n | ae1 IH1 ae2 IH2 | ae1 IH1 ae2 IH2]. *)
+(*   - rewrite fold_unfold_evaluate_v0_Literal. *)
+(*     rewrite fold_unfold_compile_v0_aux_Literal. *)
+(*     rewrite fold_unfold_fetch_decode_execute_loop_v0_cons. *)
+(*     unfold decode_execute_v0. *)
+(*     rewrite fold_unfold_fetch_decode_execute_loop_v0_nil. *)
+(*     reflexivity. *)
+(*   - rewrite fold_unfold_evaluate_v0_Plus. *)
+(*     rewrite IH1. *)
+(*     rewrite IH2. *)
+(*     rewrite fold_unfold_compile_v0_aux_Plus. *)
+(*     rewrite fetch_decode_execute_loop_v0_and_append_commute. *)
+
+(* ********** *)
+
+(* end of term-project.v *)
